\documentclass[12pt]{article}
\usepackage[left=3cm,right=3cm,top=1cm,bottom=2cm]{geometry}
\usepackage{amsmath,amsthm}
\usepackage{lipsum}
\usepackage{amssymb}
\usepackage{stmaryrd}
\usepackage{tikz}
\usepackage{pgfplots}
\usepackage{cancel}
\usepackage[T1,T2A]{fontenc}
\usepackage[utf8]{inputenc}
\usepackage[bulgarian]{babel}
\usepackage[normalem]{ulem}
    
\newcommand{\R}{\mathbb{R}}
\newcommand\tab[1][1cm]{\hspace*{#1}}

\setlength{\parindent}{0mm}
        
\title{Курсова задача №2}
\author{Иво Стратев}
        
\begin{document}
\maketitle

$f(x) = \frac{x^2 - 4}{x}.e^{-\frac{5}{3x}} = (x - \frac{4}{x})e^{-\frac{5}{3x}}$ \\

1. Допустимо множество \\

$x \in \R \backslash \{0\}$ \\\\

$\forall x \in \R \backslash \{0\} \; e^{-\frac{5}{3x}} > 0 \implies f(x) = 0 \iff \frac{x^2 - 4}{x} = 0 \iff x^2 - 4 = 0 \iff x = \pm 2$ \\\\

2. $f'(x) = (1 + \frac{4}{x^2})e^{-\frac{5}{3x}} + (x - \frac{4}{x})e^{-\frac{5}{3x}}\frac{5}{3x^2} = \\\\
= (1 + \frac{4}{x^2} + \frac{5}{3x} - \frac{20}{3x^3})e^{-\frac{5}{3x}} \\\\
\forall x \in \R \backslash \{0\} \; e^{-\frac{5}{3x}} > 0 \implies f'(x) = 0 \iff 1 + \frac{4}{x^2} + \frac{5}{3x} - \frac{20}{3x^3} = 0 \iff \\\\
\frac{3x^3 + 12x + 5x^2 - 20}{3x^3} = 0 \iff 3x^3 + 5x^2 + 12x - 20 = 0 $ \\\\

Нека $p(x) = 3x^3 + 5x^2 + 5x^2 - 20 \implies sign(f(x)) = sign(p(x)).sign(x^3)  \\\\
p(1) = 3 + 5 + 12 - 20 = 20 - 20 = 0 \implies (x - 1) \; | \; p(x) \\\\
\tab 3x^3 + 5x^2 + 12x - 20 \; : \; x - 1 = 3x^2 + 8x + 20 \\
- \\
\tab 3x^3 - 3x^2 \\
\tab \noindent\rule{4.1cm}{0.4pt} \\\\
\tab \tab \; \; \; 8x^2 + 12x - 20 \\
\tab - \\
\tab \tab \; \; \; 8x^2 - 8x \\
\tab \tab \; \; \; \noindent\rule{2.7cm}{0.4pt} \\\\
\tab \tab \tab \; \; \; 20x - 20 \\
\tab \tab - \\
\tab \tab \tab \; \; \; 20x - 20 \\
\tab \tab \; \; \; \noindent\rule{2.7cm}{0.4pt} \\\\
\tab \tab \tab \tab \; \; \; 0 \\\\
\implies p(x) = (x - 1)(3x^2 + 8x + 20)$ \\\\

Нека $q(x) = 3x^2 + 8x + 20 \\\\
D(q) = 64 - 240 < 0 \; \land \; 3 > 0 \implies \forall x \in \R \; q(x) > 0 \implies \\\\
sign(f'(x)) = sign(x - 1).sign(x^3)$ \\\\

\begin{tikzpicture}
    \draw(0,0) -- (6,0);
    \draw (2 cm,3pt) -- (2 cm,-3pt);
    \draw (4 cm,3pt) -- (4 cm,-3pt);
    \draw (0,0) node[left=3pt] {$f'(x)$};
    \draw (1,0) node[above=3pt] {$+$};
    \draw (2,0) node[] {$\times$};
    \draw (2,0) node[above=3pt] {$0$};
    \draw (3,0) node[above=3pt] {$-$};
    \draw (4,0) node[above=3pt] {$1$};
    \draw (5,0) node[above=3pt] {$+$};
\end{tikzpicture} \quad $\implies$ \quad \begin{tikzpicture}
    \draw(0,0) -- (6,0);
    \draw (2 cm,3pt) -- (2 cm,-3pt);
    \draw (4 cm,3pt) -- (4 cm,-3pt);
    \draw (0,0) node[left=3pt] {$f'(x)$};
    \draw (1,0) node[above=3pt] {$\nearrow$};
    \draw (2,0) node[] {$\times$};
    \draw (2,0) node[above=3pt] {$0$};
    \draw (3,0) node[above=3pt] {$\searrow$};
    \draw (4,0) node[above=3pt] {$1$};
    \draw (5,0) node[above=3pt] {$\nearrow$};
\end{tikzpicture} \\\\

3. \\

\begin{center}
\begin{tabular}{||l | c | c | c | c | c | c||} 
\hline
$x$ & $-\infty$ & $0-0$ & $0$ & $0 + 0$ & $1$ & $\infty$ \\ [0.5ex]
\hline\hline
$f(x)$ & $-\infty \nearrow$ & $\infty \nearrow$ & $||$ & $0 \searrow$ & $-\frac{3}{e^{\frac{5}{3}}}$ & $\infty \nearrow$ \\
\hline
$f'(x)$ & $+$ & $+$ & $||$ & $-$ & $0$ & $+$ \\
\hline
\end{tabular}
\end{center}


$f(1) = (1 - 4)e^{-\frac{5}{3}} = -\frac{3}{e^{\frac{5}{3}}} \approx -0.56663 \\\\
\forall x \in (0.5, \; 1) \; sign(f(x)) < 0 \; \land \; \forall x \in (1, \; 1.5) \; sign(f(x)) > 0 \; \land \; f(1) = 0 \implies $ \\\\
$f(1)$ е локален минимум. \\\\ 
$\lim_{x \to -\infty} f(x) = \lim_{x \to -\infty} (x - \frac{4}{x})e^{-\frac{5}{3x}}
= \left[\lim_{x \to -\infty}  (x - \frac{4}{x})\right] . \left[\lim_{x \to -\infty} e^{-\frac{5}{3x}}\right] = \\\\
= \left[\left(\lim_{x \to -\infty} x\right)  - \left(\lim_{x \to -\infty} \frac{4}{x}\right)\right] . \left[e^{\lim_{x \to -\infty}-\frac{5}{3x}}\right]
= \left[\left(\lim_{x \to -\infty} x\right)  - 0\right] . e^0 = \\\\
= \lim_{x \to -\infty} x = - \infty \\\\
\lim_{x \to \infty} f(x) = \lim_{x \to \infty} (x - \frac{4}{x})e^{\frac{5}{3x}}
= \left[\lim_{x \to \infty}  (x - \frac{4}{x})\right] . \left[\lim_{x \to \infty} e^{-\frac{5}{3x}}\right] = \\\\
= \left[\left(\lim_{x \to \infty} x\right)  - \left(\lim_{x \to \infty} \frac{4}{x}\right)\right] . \left[e^{\lim_{x \to \infty}-\frac{5}{3x}}\right]
= \left[\left(\lim_{x \to \infty} x\right)  - 0\right] . e^0 = \\\\
= \lim_{x \to \infty} x = \infty \\\\
\lim_{x \to 0 - 0} f(x) = \lim_{x \to 0 - 0} (x - \frac{4}{x})e^{-\frac{5}{3x}}
= \left[\lim_{x \to 0 - 0}  (x - \frac{4}{x})\right] . \left[\lim_{x \to 0 - 0} e^{-\frac{5}{3x}}\right] = \\\\
= \left[\left(\lim_{x \to 0 - 0} x\right)  - \left(\lim_{x \to 0 - 0} \frac{4}{x}\right)\right] . \left[e^{\lim_{x \to 0 - 0}-\frac{5}{3x}}\right]
= \left[0^- - (-\infty)\right] . \left[e^\infty\right] = \\\\
= \infty.\infty = \infty \\\\
\lim_{x \to 0 + 0} f(x) = \lim_{x \to 0 + 0} (x - \frac{4}{x})e^{-\frac{5}{3x}}
= \left[\lim_{x \to 0 + 0} \frac{x}{e^{\frac{5}{3x}}}\right] - 4\left[\lim_{x \to 0 + 0}\frac{\frac{1}{x}}{e^{\frac{5}{3x}}}\right] \\\\
\lim_{x \to 0 + 0} \frac{x}{e^{\frac{5}{3x}}} = \lim_{x \to 0 + 0} \frac{1}{\frac{1}{x}e^{\frac{5}{3x}}}
= \frac{1}{\left[\lim_{x \to 0 + 0}\frac{1}{x}\right]\left[\lim_{x \to 0 + 0}e^{\frac{5}{3x}}\right]} = \frac{1}{\infty.\infty} = \frac{1}{\infty} = 0 \\\\\\
\lim_{x \to 0 + 0}\frac{\frac{1}{x}}{e^{\frac{5}{3x}}} = \frac{\infty}{\infty} \implies
\lim_{x \to 0 + 0}\frac{\frac{1}{x}}{e^{\frac{5}{3x}}} = \lim_{x \to 0 + 0}\frac{-\frac{1}{x^2}}{e^{\frac{5}{3x}}.\left(-\frac{5}{3x^2}\right)} = \\\\
= \lim_{x \to 0 + 0}\frac{3}{5e^{\frac{5}{3x}}} = \frac{3}{5}\frac{1}{e^{\lim_{x \to 0 + 0}\frac{5}{3x}}}
= \frac{3}{5}\frac{1}{e^\infty} = \frac{3}{5}\frac{1}{\infty} = \frac{3}{5}.0 = 0 \implies \\\\
\lim_{x \to 0 + 0} f(x) = 0 - 4.0 = 0 - 0 = 0$ \\\\

\begin{tikzpicture}
    \draw[->] (-8.5,0) -- (8.5,0) node[right] {$x$};
  \draw[->] (0,-8.5) -- (0,8.5) node[above] {$f(x)$};
  \draw(-8.5,-8.5) -- (-0.1, 8.5);
  \draw(0.01, 0) -- (0.5, -0.2);
  \draw(0.5, -0.2) -- (8.5, 5.5);
\end{tikzpicture} \\\\

4. $f''(x) = \left[\left(1 + \frac{4}{x^2} + \frac{5}{3x} - \frac{20}{3x^3}\right)e^{-\frac{5}{3x}}\right]' = \\\\
= \left(-\frac{8}{x^3} - \frac{5}{3x^2} + \frac{20}{x^4}\right)e^{-\frac{5}{3x}}
+ \left(1 + \frac{4}{x^2} + \frac{5}{3x} - \frac{20}{3x^3}\right)e^{-\frac{5}{3x}}.\left(\frac{5}{3x^2}\right) = \\\\
= e^{-\frac{5}{3x}}\left(-\frac{8}{x^3} - \frac{5}{3x^2} + \frac{20}{x^4} + \frac{5}{3x^2} + \frac{20}{3x^4} + \frac{25}{9x^3} - \frac{100}{9x^5}\right) = \\\\
= e^{-\frac{5}{3x}}\left(-\frac{47}{9x^3} + \frac{80}{3x^4} - \frac{100}{9x^5}\right) = e^{-\frac{5}{3x}}\left(-\frac{47x^2 - 240x + 100}{9x^5}\right) \\\\
\forall x \in \R \backslash \{0\} \; e^{-\frac{5}{3x}} > 0 \implies f''(x) = 0 \iff \frac{47x^2 - 240x + 100}{9x^5} = 0 \iff \\\\
47x^2 - 240x + 100 = 0$ \\\\

Нека $g(x) = 47x^2 - 240x + 100 \implies sign(f''(x)) = sign(g(x)).sign(x^5) = sign(x).sign(g(x)) \\\\
D(g) = 240^2 - 47.400 = 400(24.6 - 47) = \\\\
= 400(144 - 47) = 400.97 = 20^2.97 \implies \sqrt{D(g)} = 20\sqrt{97} \implies \\\\
x_{1, \; 2} = \frac{240 \pm 20\sqrt{97}}{2.47} = \frac{120 \mp 10 \sqrt{97}}{47} = \frac{10}{47}(12 \mp \sqrt{97}) \approx 2.5532 \mp 2.0955 \implies \\\\
x_1 \approx 0.4577 \; , \quad x_2 \approx 4.6487 \implies \\\\
sign(f''(x)) = sign(x).sign(-(x - x_1)(x + x_2)) = -sign(x).sign((x - x_1)(x - x_2))$ \\\\

$\implies$ \quad \begin{tikzpicture}
    \draw(0,0) -- (8,0);
    \draw (2 cm,3pt) -- (2 cm,-3pt);
    \draw (4 cm,3pt) -- (4 cm,-3pt);
    \draw (6 cm,3pt) -- (6 cm,-3pt);
    \draw (0,0) node[left=3pt] {$f'(x)$};
    \draw (1,0) node[above=3pt] {$+$};
    \draw (2,0) node[] {$\times$};
    \draw (2,0) node[above=3pt] {$0$};
    \draw (3,0) node[above=3pt] {$-$};
    \draw (4,0) node[above=3pt] {$x_1$};
    \draw (5,0) node[above=3pt] {$+$};
    \draw (6,0) node[above=3pt] {$x_2$};
    \draw (7,0) node[above=3pt] {$-$};
\end{tikzpicture} \\\\
$\implies$ \quad \begin{tikzpicture}
    \draw(0,0) -- (8,0);
    \draw (2 cm,3pt) -- (2 cm,-3pt);
    \draw (4 cm,3pt) -- (4 cm,-3pt);
    \draw (6 cm,3pt) -- (6 cm,-3pt);
    \draw (0,0) node[left=3pt] {$f'(x)$};
    \draw (1,0) node[above=3pt] {$\smile$};
    \draw (2,0) node[] {$\times$};
    \draw (2,0) node[above=3pt] {$0$};
    \draw (3,0) node[above=3pt] {$\frown$};
    \draw (4,0) node[above=3pt] {$x_1$};
    \draw (5,0) node[above=3pt] {$\smile$};
    \draw (6,0) node[above=3pt] {$x_2$};
    \draw (7,0) node[above=3pt] {$\frown$};
\end{tikzpicture} \\\\

5. \\

\begin{center}
    \begin{tabular}{||l | c | c | c | c | c | c | c | c||} 
    \hline
    $x$ & $-\infty$ & $0-0$ & $0$ & $0 + 0$ & $x_1$ & $1$ & $x_2$ & $\infty$ \\ [0.5ex]
    \hline\hline
    $f(x)$ & $-\infty \; \nearrow \; \smile$ & $\infty \; \nearrow \; \smile$ & $||$ & $0 \; \searrow \; \frown$ & $f(x_1)$ & $-\frac{3}{e^{\frac{5}{3}}}$ & $f(x_2)$ & $\infty \; \nearrow \; \frown$ \\
    \hline
    $f'(x)$ & $+$ & $+$ & $||$ & $-$ & $f'(x_1)$ & $0$ & $f'(x_2)$ & $+$ \\
    \hline
    $f''(x)$ & $+$ & $+$ & $||$ & $-$ & $0$ & $+$ & $0$ & $-$ \\
    \hline
\end{tabular}
\end{center}

$f(x_1) = f(\frac{10}{47}(12 - \sqrt{97})) = \left(\frac{10}{47}(12 - \sqrt{97}) - \frac{94}{5(12 - \sqrt{97})}\right)e^{-\frac{47}{6(12 - \sqrt{97})}} \approx -0.21709732 \\\\
f(x_2) = f(\frac{10}{47}(12 + \sqrt{97})) = \frac{48}{235}(-11 + 3\sqrt{97})e^{-2 + \frac{\sqrt{97}}{6}} \approx 2.64686745142 \\\\
f'(x_1) = f'(\frac{10}{47}(12 - \sqrt{97})) = -\frac{2}{25}(277 + 30\sqrt{97})e^{-2 - \frac{\sqrt{97}}{6}} \approx -1.20051176 \\\\
f'(x_2) = f'(\frac{10}{47}(12 + \sqrt{97})) = \frac{2}{25}(30\sqrt{97} - 277)e^{\frac{\sqrt{97}}{6} - 2} \approx 1.0321711097 \\\\
((T_1(f))(a))(x) = f(a) + f'(a)(x - a) \implies \\\\
((T_1(f))(x_1))(x) = f(x_1) + f'(x_1)(x - x_1) \\\\
((T_1(f))(x_2))(x) = f(x_2) + f'(x_2)(x - x_2) \\\\
((T_1(f))(1))(x) = f(1) + f'(1)(x - a) = f(1) + 0 = -\frac{3}{e^{\frac{5}{3}}} \approx -0.5666268085\\\\
((T_1(f))(-2))(x) = f(-2) + f'(-2)(x + 2) = 0 + (1 + 1 - \frac{5}{6} + \frac{5}{6})e^{\frac{5}{6}} = 2e^{\frac{5}{6}}(x + 2) \\\\
((T_1(f))(2))(x) = f(2) + f'(2)(x - 2) = 0 + (1 + 1 + \frac{5}{6} - \frac{5}{6})e^{\frac{5}{6}} = 2e^{-\frac{5}{6}}(x - 2)$ \\\\

\begin{tikzpicture}
\begin{axis}[
    ticks=none,
    width=\textwidth,
    samples=2000,
    domain=-20:20,
    restrict y to domain =-20:20,
    axis x line=center,
    axis y line=center,
    xmin=-20,
    xmax=20,
    ymin=-20,
    ymax=20,
    xlabel={$x$},
    ylabel={$f(x)$},
    legend pos=south east]
]
\addplot[no markers, solid, smooth, red] plot (\x, {(\x - 4/\x) * exp((-5)/(3 * \x)});
\legend{$f(x) = (x - \frac{4}{x})e^{-\frac{5}{3x}}$}
\end{axis}
\end{tikzpicture} \\\\


\begin{tikzpicture}
    \begin{axis}[
        ticks=none,
        width=\textwidth,
        samples=2000,
        domain=-20:20,
        restrict y to domain =-20:20,
        axis x line=center,
        axis y line=center,
        xmin=-20,
        xmax=20,
        ymin=-20,
        ymax=20,
        xlabel={$x$},
        ylabel={$f(x)$},
        legend pos=south east]
    ]
    \addplot[no markers, solid, smooth, red] plot (\x, {(\x - 4/\x) * exp((-5)/(3 * \x)});
    \addplot[no markers, solid, smooth, cyan] plot (\x, {exp(-5/(3 * \x)) * (-20 + 12 * \x + 5 * \x^2 + 3 * \x^3))/(3 * \x^3)});
    \addplot[no markers, solid, smooth, green] plot (\x, {-1 * exp(-5/(3 * \x)) * ((47 * \x^2 - 240 * \x + 100)/(9 * \x^5))});
    \legend{$f(x)$,$f'(x)$,$f''(x)$}
\end{axis}
\end{tikzpicture} \\\\


\begin{tikzpicture}
    \begin{axis}[
        ticks=none,
        width=\textwidth,
        samples=2000,
        domain=-20:20,
        restrict y to domain =-20:20,
        axis x line=center,
        axis y line=center,
        xmin=-20,
        xmax=20,
        ymin=-20,
        ymax=20,
        xlabel={$x$},
        ylabel={$f(x)$},
        legend pos=south east]
    \pgfmathsetmacro{\s}{10/47 * (12 - sqrt(97))};
    \pgfmathsetmacro{\fs}{-0.21709732};
    \pgfmathsetmacro{\dfs}{-1.20051176};
    \pgfmathsetmacro{\t}{10/47 * (12 + sqrt(97))};
    \pgfmathsetmacro{\ft}{2.64686745142};
    \pgfmathsetmacro{\dft}{1.0321711097};
    \addplot[no markers, solid, smooth, violet] plot (\x, {(\x - 4/\x) * exp((-5)/(3 * \x)});
    \addplot[no markers, solid, smooth, green] plot (\x, {2 * exp(5 / 6) * (\x + 2)});
    \addplot[no markers, solid, smooth, orange] plot (\x, {2 / exp(5 / 6) * (\x - 2)});
    \addplot[no markers, solid, smooth, blue] plot (\x, {-3/(exp(5/3))});
    \addplot[no markers, solid, smooth, magenta] plot (\x, {\fs + \dfs * (\x - \s)});
    \addplot[no markers, solid, smooth, cyan] plot (\x, {\ft + \dft * (\x - \t)});
    \legend{$f(x)$,$((T_1(f))(-2))(x)$,$((T_1(f))(2))(x)$,$((T_1(f))(1))(x)$,$((T_1(f))(x_1))(x)$,$((T_1(f))(x_2))(x)$}
    \end{axis}
\end{tikzpicture} \\\\


\begin{tikzpicture}
    \begin{axis}[
        ticks=none,
        width=\textwidth,
        samples=2000,
        domain=-5:5,
        restrict y to domain =-5:5,
        axis x line=center,
        axis y line=center,
        xmin=-5,
        xmax=5,
        ymin=-5,
        ymax=5,
        xlabel={$x$},
        ylabel={$f(x)$},
        legend pos=south east]
    \pgfmathsetmacro{\s}{10/47 * (12 - sqrt(97))};
    \pgfmathsetmacro{\fs}{-0.21709732};
    \pgfmathsetmacro{\dfs}{-1.20051176};
    \pgfmathsetmacro{\t}{10/47 * (12 + sqrt(97))};
    \pgfmathsetmacro{\ft}{2.64686745142};
    \pgfmathsetmacro{\dft}{1.0321711097};
    \addplot[no markers, solid, smooth, violet] plot (\x, {(\x - 4/\x) * exp((-5)/(3 * \x)});
    \addplot[no markers, solid, smooth, green] plot (\x, {2 * exp(5 / 6) * (\x + 2)});
    \addplot[no markers, solid, smooth, orange] plot (\x, {2 / exp(5 / 6) * (\x - 2)});
    \addplot[no markers, solid, smooth, blue] plot (\x, {-3/(exp(5/3))});
    \addplot[no markers, solid, smooth, magenta] plot (\x, {\fs + \dfs * (\x - \s)});
    \addplot[no markers, solid, smooth, cyan] plot (\x, {\ft + \dft * (\x - \t)});
    \legend{$f(x)$,$((T_1(f))(-2))(x)$,$((T_1(f))(2))(x)$,$((T_1(f))(1))(x)$,$((T_1(f))(x_1))(x)$,$((T_1(f))(x_2))(x)$}
    \end{axis}
\end{tikzpicture} \\\\

\begin{tikzpicture}
    \begin{axis}[
        ticks=none,
        width=\textwidth,
        samples=2000,
        domain=-5:5,
        restrict y to domain =-5:5,
        axis x line=center,
        axis y line=center,
        xmin=-5,
        xmax=5,
        ymin=-5,
        ymax=5,
        xlabel={$x$},
        ylabel={$f(x)$},
        legend pos=south east]
    \pgfmathsetmacro{\s}{10/47 * (12 - sqrt(97))};
    \pgfmathsetmacro{\fs}{-0.21709732};
    \pgfmathsetmacro{\dfs}{-1.20051176};
    \pgfmathsetmacro{\t}{10/47 * (12 + sqrt(97))};
    \pgfmathsetmacro{\ft}{2.64686745142};
    \pgfmathsetmacro{\dft}{1.0321711097};
    \addplot[no markers, solid, smooth, violet] plot (\x, {(\x - 4/\x) * exp((-5)/(3 * \x)});
    \addplot[no markers, solid, smooth, lime] plot (\x, {exp(-5/(3 * \x)) * (-20 + 12 * \x + 5 * \x^2 + 3 * \x^3))/(3 * \x^3)});
    \addplot[no markers, solid, smooth, yellow] plot (\x, {-1 * exp(-5/(3 * \x)) * ((47 * \x^2 - 240 * \x + 100)/(9 * \x^5))});
    \addplot[no markers, solid, smooth, green] plot (\x, {2 * exp(5 / 6) * (\x + 2)});
    \addplot[no markers, solid, smooth, orange] plot (\x, {2 / exp(5 / 6) * (\x - 2)});
    \addplot[no markers, solid, smooth, blue] plot (\x, {-3/(exp(5/3))});
    \addplot[no markers, solid, smooth, magenta] plot (\x, {\fs + \dfs * (\x - \s)});
    \addplot[no markers, solid, smooth, cyan] plot (\x, {\ft + \dft * (\x - \t)});
    \legend{$f(x)$,$f'(x)$,$f''(x)$,$((T_1(f))(-2))(x)$,$((T_1(f))(2))(x)$,$((T_1(f))(1))(x)$,$((T_1(f))(x_1))(x)$,$((T_1(f))(x_2))(x)$}
    \end{axis}
\end{tikzpicture}

\end{document}